Add a bunch of module stuff, and update to new coq/math-classes.

module.v
@@ -1,13 +1,13 @@
 Require Import
-   Morphisms RelationClasses Equivalence Setoid
-   abstract_algebra setoid.
+   Morphisms RelationClasses Equivalence Setoid Program
+   abstract_algebra varieties.setoid semigroup.
 Require Import rings.
 
 (* me *)
 
 Require Import extra_tactics.
 
-Set Implicit Arguments.
+(*Set Implicit Arguments.*)
 
 Infix "<*>" := ralgebra_action (at level 30).
 
@@ -22,33 +22,20 @@ Class Rmodule `(ez: Equiv Scalar) `(ee: Equiv Elem) `{op: RalgebraAction Scalar 
   ; rmodule_distr_r: `((x + y) <*> a = (x <*> a) & (y <*> a))
   ; rmodule_assoc: `((x * y) <*> a = x <*> (y <*> a)) }.
 
+Ungereralizable Arguments  Rmodule [ez szalar_plus szalar_mult szalar_zero szalar_one szalar_inv].
+
 Class Ralgebra `(ez: Equiv Scalar) `(e': Equiv Elem) `{RalgebraAction Scalar Elem}
     szalar_plus szalar_mult szalar_inv szalar_zero szalar_one
     elem_plus elem_mult elem_zero elem_one elem_opp: Prop :=
   { ralgebra_module:> Rmodule ez e'
       szalar_plus szalar_mult szalar_inv szalar_zero szalar_one
       elem_plus elem_zero elem_opp
-  ; ralgebra_ring:> @Ring Elem e' elem_plus elem_mult elem_zero elem_one elem_opp
+  ; ralgebra_ring: @Ring Elem e' elem_plus elem_mult elem_zero elem_one elem_opp
   ; ralgebra_assoc: `(x <*> (a * b) = (x <*> a) * b) }.
 
-Section Morphisms.
-Context `{Ring R} `{Rmodule R M} {r: R}.
-Global Instance: Setoid_Morphism (ralgebra_action r).
-Global Instance: SemiGroup_Morphism (ralgebra_action r).
-Proof.
-  intuition; constructor; try typeclasses eauto.
-  apply rmodule_distr_l.
-Qed.
-Global Instance: Monoid_Morphism (ralgebra_action r).
-Proof.
-  intuition constructor; try typeclasses eauto.
-  apply (right_cancel (r<*>-mon_unit)).
-  rewrite left_identity.
-  rewrite <- rmodule_distr_l.
-  rewrite left_identity.
-  apply rmodule_action_proper; try reflexivity.
-Qed.
-
+Implicit Arguments left_cancellation [[A][e][op][LeftCancellation]].
+Implicit Arguments right_cancellation [[A][e][op][RightCancellation]].
+(*
 Global Instance SemiGroup_Morphism_id M `{SemiGroup M}: SemiGroup_Morphism (id: M→M).
 Proof.
   constructor; try typeclasses eauto.
@@ -56,9 +43,26 @@ Proof.
 Qed.
 Global Instance Monoid_Morphism_id M `{Monoid M} : Monoid_Morphism (id: M→M).
 Proof. constructor; try typeclasses eauto; reflexivity. Qed.
+*)
 
-Require Import Program.
-Require Import setoids.
+Section Morphisms.
+Context `{Ring R} `{Rmodule R M} {r: R}.
+Global Instance: SemiGroup_Morphism (ralgebra_action r).
+Proof.
+  intuition constructor; try typeclasses eauto.
+  constructor; try typeclasses eauto.
+  apply rmodule_distr_l.
+Qed.
+Global Instance: Monoid_Morphism (ralgebra_action r).
+Proof.
+  intuition constructor; try typeclasses eauto.
+  apply (right_cancellation (r<*>-mon_unit)).
+  rewrite left_identity.
+  rewrite <- rmodule_distr_l.
+  rewrite left_identity.
+  apply rmodule_action_proper; try reflexivity.
+Qed.
+
 Global Instance SemiGroup_Morphism_comp
     S T U `{SemiGroup S} `{SemiGroup T} `{SemiGroup U} (f: T→U) (g: S→T)
     `{!SemiGroup_Morphism f} `{!SemiGroup_Morphism g}
@@ -83,7 +87,7 @@ Section Basic_Lemmas.
 Context `{Ring R} `{Rmodule R M}.
 Lemma rmodule_zero_action r: (0 <*> r = mon_unit).
 Proof.
-  apply (left_cancel (1<*>r)).
+  apply (left_cancellation (1<*>r)).
   rewrite <- rmodule_distr_r.
   rewrite (right_identity (1<*>r)).
   apply rmodule_action_proper; try reflexivity.
@@ -92,9 +96,9 @@ Qed.
 Lemma rmodule_minus: `((-r) <*> m = -r <*> m).
 Proof.
   intros r m.
-  apply inv_unique; left.
+  apply (left_cancellation (r<*>m)).
   rewrite <- (rmodule_distr_r).
-  rewrite plus_opp_r.
+  do 2 rewrite right_inverse.
   apply rmodule_zero_action.
 Qed.
 End Basic_Lemmas.
@@ -102,7 +106,7 @@ End Basic_Lemmas.
 
 Section Rmodules.
 
-Class Rmodule_Morphism Scalar M1 M2 {ez: Equiv Scalar} {e1: Equiv M1} `{RalgebraAction Scalar M1} {e2: Equiv M2} `{RalgebraAction Scalar M2}
+Class Rmodule_Morphism {Scalar M1 M2: Type} {ez: Equiv Scalar} {e1: Equiv M1} `{RalgebraAction Scalar M1} {e2: Equiv M2} `{RalgebraAction Scalar M2}
     {szalar_plus} {szalar_mult} {szalar_zero: RingZero Scalar} {szalar_one: RingOne Scalar} {szalar_inv: GroupInv Scalar}
     {M1_plus} {M1_zero} {M1_opp} {M2_plus} {M2_zero} {M2_opp} (f: M1 -> M2) :=
 { rmodule_morphism_ring : @Ring Scalar ez szalar_plus szalar_mult szalar_zero szalar_one szalar_inv
@@ -190,14 +194,16 @@ Proof. intro; reflexivity. Qed.
 
 Global Instance: Category Object := { comp_assoc := comp_assoc'; id_l := id_l'; id_r := id_r'}.
 
+End Rmodules.
+
 Section Kernel.
 Context {M N: Type}.
 
 (* TODO: This should be in terms of pointed setoids. *)
 Context `{Monoid M, Monoid N} (f: M→N) `{!Monoid_Morphism f}.
 Definition Kernel := {m: M | f m = mon_unit}.
-Global Instance e: Equiv Kernel := fun k k' => `k = `k'.
-Instance: Equivalence e.
+Global Instance ee: Equiv Kernel := fun k k' => `k = `k'.
+Instance: Equivalence ee.
 Global Instance: Setoid Kernel.
 Global Program Instance Kop: SemiGroupOp Kernel := fun k k' => exist _ (`k & `k') _.
 Next Obligation.
@@ -206,27 +212,27 @@ Next Obligation.
   rewrite Hk, Hk'.
   apply left_identity.
 Qed.
-Global Instance: Proper (e==>e==>e) sg_op.
+Global Instance: Proper (ee==>ee==>ee) sg_op.
 Proof.
   intros [??][??]?[??][??]?.
-  unfold e; simpl.
+  unfold ee; simpl.
   apply sg_mor; assumption.
 Qed.
 Global Instance: Associative Kop.
 Proof.
   intros [??][??][??].
-  unfold equiv, e, Kop; simpl.
+  unfold equiv, ee, Kop; simpl.
   apply (sg_ass _).
 Qed.
 Global Instance: SemiGroup Kernel.
 Global Program Instance: MonoidUnit Kernel := exist _ mon_unit preserves_mon_unit.
 Global Instance: LeftIdentity Kop mon_unit.
-Proof. intros [??]; unfold equiv, e, mon_unit, MonoidUnit_instance_0; simpl; apply left_identity. Qed.
+Proof. intros [??]; unfold equiv, ee, mon_unit, MonoidUnit_instance_0; simpl; apply left_identity. Qed.
 Global Instance: RightIdentity Kop mon_unit.
-Proof. intros [??]; unfold equiv, e, mon_unit, MonoidUnit_instance_0; simpl; apply right_identity. Qed.
+Proof. intros [??]; unfold equiv, ee, mon_unit, MonoidUnit_instance_0; simpl; apply right_identity. Qed.
 Global Instance: Monoid Kernel.
 Let  i: Kernel→M := @projT1 _ _.
-Global Instance: Proper (e==>equiv) i.
+Global Instance: Proper (equiv==>equiv) i.
 Proof. intros [??][??]?; unfold i; simpl; assumption. Qed.
 Global Instance x(*TODO: Name?*): Setoid_Morphism (@projT1 _ _:Kernel->M).
 Global Instance: SemiGroup_Morphism (@projT1 _ _:Kernel->M).
@@ -240,7 +246,7 @@ Proof.
 Qed.
 Context `{!Commutative sg_op}.
 Global Instance: Commutative (A:=Kernel) sg_op.
-Proof. intros [??][??]; unfold equiv, e; simpl; apply commutativity. Qed.
+Proof. intros [??][??]; unfold equiv, ee. simpl; apply commutativity. Qed.
 End Kernel.
 
 Section Kernel_Group.
@@ -250,15 +256,15 @@ Global Program Instance: GroupInv (Kernel f) := fun k => exist _ (-`k) _.
 Next Obligation.
   destruct k as [k Hk]; simpl.
   rewrite preserves_inv, Hk; try typeclasses eauto.
-  exact inv_zero.
+  exact inv_0.
 Qed.
 Global Instance: Proper (equiv==>equiv) (group_inv (A:=Kernel f)).
-Proof. intros [??][??]?; unfold equiv, e; simpl; apply inv_proper; assumption. Qed.
+Proof. intros [??][??]?; unfold equiv, ee; simpl; apply inv_proper; assumption. Qed.
 (* TODO: Define LeftInverse and RightInverse classes. *)
 Global Instance Kernel_Group: Group `{Kernel f}.
 Proof.
   constructor; try typeclasses eauto
-  ; intros [??]; unfold equiv, e; simpl; [apply ginv_l | apply ginv_r].
+  ; intros [??]; unfold equiv, ee; simpl; [apply ginv_l | apply ginv_r].
 Qed.
 End Kernel_Group.
 Section Kernel_AbGroup.
@@ -277,7 +283,7 @@ Next Obligation.
 Qed.
 Global Instance: !Rmodule R (Kernel f).
 Proof.
-  constructor; try typeclasses eauto; unfold equiv, e, Proper, "==>"; intuition;
+  constructor; try typeclasses eauto; unfold equiv, ee, Proper, "==>"; intuition;
     repeat match goal with
       | [ x : Kernel f |- _ ] => destruct x
     end; simpl.
@@ -296,6 +302,429 @@ Qed.
 
 End Kernel_Rmodule.
 
+Inductive Cokernel `(f:M→N)  := cok { sec : N }.
+Implicit Arguments cok [[M] [N] [f]].
+Implicit Arguments sec [[M] [N] [f]].
+Section CoKernel.
+Context {M N: Type}.
 
-Context `{M: nat → Type}.
-Context `{forall n: nat, Rmodule R (e:=e) (M n)}.
+(* TODO: Define this more generally *)
+Context `{AbGroup M, AbGroup N} (f: M→N) `{!Monoid_Morphism f}.
+Local Notation Cokernel := (Cokernel f).
+Global Instance eck: Equiv Cokernel := fun x y => ∃ k: M, sec x = f(k) & sec y.
+Global Instance: Equivalence eck.
+Proof. constructor.
+  * intro x; exists mon_unit.
+    rewrite preserves_mon_unit, left_identity; reflexivity.
+  * intros x y [k Hk]; exists (-k).
+    rewrite preserves_inv; try typeclasses eauto.
+    apply (left_cancellation (f k)).
+    rewrite <- Hk, sg_ass, ginv_r, left_identity; try typeclasses eauto.
+    reflexivity.
+  * intros x y z [k Hk] [k' Hk'].
+    exists (k & k').
+    rewrite preserves_sg_op, Hk, Hk', sg_ass; try typeclasses eauto.
+    reflexivity.
+Qed.
+Global Instance: Setoid Cokernel.
+Global Instance: Proper (equiv ==> equiv) cok.
+Proof.
+  intros ???. exists mon_unit. simpl.
+  rewrite preserves_mon_unit, left_identity; assumption.
+Qed.
+Global Instance Setoid_Morphism_instance_1: Setoid_Morphism (cok:N→Cokernel).
+Global Instance: SemiGroupOp Cokernel := fun x y => cok (sec x & sec y).
+Global Instance: Associative (A:=Cokernel) sg_op.
+Proof.
+  intros x y z. 
+  exists mon_unit.
+  rewrite preserves_mon_unit, left_identity.
+  destruct x, y, z. simpl.
+  apply sg_ass.
+  typeclasses eauto.
+Qed.
+Global Instance: Proper (equiv==>equiv==>equiv) (sg_op:_->_->Cokernel).
+Proof.
+  intros [?][?][k Hk] [?][?][k' Hk']. 
+  exists (k & k'); simpl.
+  setoid_rewrite Hk.  setoid_rewrite Hk'.
+  rewrite <- sg_ass at 1 by typeclasses eauto.
+  setoid_rewrite sg_ass at 2; try typeclasses eauto.
+  setoid_rewrite commutativity at 3. simpl.
+  repeat rewrite sg_ass by typeclasses eauto.
+  rewrite <- preserves_sg_op, <- sg_ass.
+  reflexivity.
+  typeclasses eauto.
+Qed.
+Global Instance: Commutative (A:=Cokernel) sg_op.
+Proof.
+  intros x y.
+  destruct x, y.
+  exists mon_unit; rewrite preserves_mon_unit, left_identity.
+  simpl; apply commutativity.
+Qed.
+Global Instance: SemiGroup Cokernel.
+Global Instance: SemiGroup_Morphism cok.
+Proof. constructor; try typeclasses eauto; reflexivity. Qed.
+Global Instance: MonoidUnit Cokernel := cok mon_unit.
+Global Instance: LeftIdentity sg_op (mon_unit:Cokernel).
+Proof.
+  intros [x].
+  exists mon_unit; rewrite preserves_mon_unit. 
+  simpl; reflexivity.
+Qed.
+Global Instance: RightIdentity sg_op (mon_unit:Cokernel).
+Proof.
+  intros [x].
+  exists mon_unit; rewrite preserves_mon_unit.
+  simpl.
+  rewrite left_identity.
+  apply right_identity.
+Qed.
+Global Instance: Monoid Cokernel.
+Global Instance Monoid_Morphism_1: Monoid_Morphism cok.
+Proof. constructor; try typeclasses eauto; reflexivity. Qed.
+Global Instance: GroupInv Cokernel := fun x => cok (- sec x).
+Global Instance: Proper (equiv ==> equiv) (group_inv:_->Cokernel).
+Proof.
+  intros [?][?][k Hk]; exists (-k). simpl.
+  rewrite Hk, sg_inv_distr, (preserves_inv k).
+  reflexivity.
+Qed.
+Global Instance: Group Cokernel.
+Proof.
+  constructor; try typeclasses eauto.
+  * intros [x]. exists mon_unit. rewrite preserves_mon_unit, right_identity. simpl. apply ginv_l.
+  * intros [x]. exists mon_unit. rewrite preserves_mon_unit, right_identity. simpl. apply ginv_r.
+Qed.
+Global Instance: AbGroup Cokernel.
+End CoKernel.
+Section Cokernel_Rmodule.
+Context {M N: Type}.
+Context `{Ring R} `{Rmodule R M, Rmodule R N} (f: M→N) `{!Rmodule_Morphism f}.
+(*cpdt*)
+Ltac notHyp P :=
+  match goal with
+    | [ _ : P |- _ ] => fail 1
+    | _ => idtac
+  end.
+Ltac extend pf :=
+  let t := type of pf in
+    notHyp t; generalize pf; intro.
+(*Local Hint Extern 0 AbGroup => match goal with 
+  [ x : Rmodule _ _ _ _ _ _ _ _ _ _ |- _ ] => extend (rmodule_abgroup (Rmodule:=x))
+end : typeclass_instances.*)
+(*TODO: pereformance hack *)
+Let ABM := (rmodule_abgroup (Rmodule:=H0)).
+Let ABN := (rmodule_abgroup (Rmodule:=H1)).
+Existing Instance ABM.
+Existing Instance ABN.
+(* end preformance hack *)
+Global Instance: RalgebraAction R (Cokernel f) := fun r n => cok (r <*> sec n).
+Global Instance: Proper (equiv ==> eck f ==> eck f) ralgebra_action.
+Proof.
+  intros ? r Hr [?][?][k Hk]. exists (r <*> k).
+  simpl.
+  rewrite Hk, preserves_rmodule_action; simpl.
+  rewrite <- rmodule_distr_l.
+  apply rmodule_action_proper; [assumption | reflexivity].
+Qed.
+Global Instance: !Rmodule R (ee:=eck f) (Cokernel f).
+Proof.
+  constructor; try typeclasses eauto.
+  Ltac simpl_cok := exists mon_unit; rewrite preserves_mon_unit, left_identity; simpl.
+  * intros [x]; simpl_cok. apply rmodule_unital.
+  * intros r [a] [b]; simpl_cok; apply rmodule_distr_l.
+  * intros r s [a]; simpl_cok; apply rmodule_distr_r.
+  * intros r s [a]; simpl_cok; apply rmodule_assoc.
+Qed.
+Global Instance Rmodule_Morphism_1: Rmodule_Morphism (e2:=eck f) cok.
+Proof. constructor; try typeclasses eauto; reflexivity. Qed.
+End Cokernel_Rmodule.
+
+Section Exact.
+Context {M N O: Type} `{Monoid M, Monoid N, Monoid O}.
+Context (f: M→N) (g: N→O) `{!Monoid_Morphism f, !Monoid_Morphism g}.
+
+Class Exact: Type := (* FIXME: Type *)
+{ image_in_kernel : ∀ m, g (f m) = mon_unit
+; kernel_in_image : ∀ n, g n = mon_unit → ∃ m , f m = n
+}.
+Class Mono: Prop := mono: ∀ m m', f m = f m' → m = m'.
+Class Epi: Prop := epi: ∀ o, ∃ m, g m = o.
+Class ShortExact :=
+{ exact1 : Mono
+; exact2 : Exact
+; exact3 : Epi
+}.
+
+Lemma mono_preserves_unit `{Mono}: ∀ m, f m = mon_unit → m = mon_unit.
+Proof.
+  intros m Hm.
+  apply mono.
+  rewrite preserves_mon_unit; assumption.
+Qed.
+End Exact.
+Section Exact2.
+Context {M N O: Type} `{AbGroup M, AbGroup N, AbGroup O}.
+Context (f: M→N) (g: N→O) `{!Monoid_Morphism f, !Monoid_Morphism g}.
+Context `{!Exact f g}.
+(* FIXME: naming *)
+Lemma exact_equal_epi n n': g n = g n' ↔ ∃ m, n = f m & n'.
+Proof.
+  split.
+  * intro Hn.
+    assert (g (n & -(n')) = mon_unit).
+    rewrite preserves_sg_op, Hn, <- preserves_sg_op.
+    rewrite ginv_r.
+    apply preserves_mon_unit.
+    set (m := kernel_in_image f g (n & -n')).
+    destruct m as [m Hm]; [assumption | exists m].
+    rewrite Hm, <- sg_ass, ginv_l, right_identity; try typeclasses eauto.
+    reflexivity.
+  * intros [m Hm].
+    rewrite Hm.
+    rewrite preserves_sg_op.
+    rewrite <- (left_identity (g n')) at 2.
+    apply sg_mor; [| reflexivity ].
+    apply (image_in_kernel f g m).
+Qed.
+End Exact2.
+
+Tactic Notation "unfold_equiv" "in" hyp(H) :=
+  match type of H with
+    | context ctx [@equiv ?A ?eq ?a ?b ]  =>
+      let T := eval red in (@equiv A eq a b) in
+      let T := eval red in T in
+        let new := context ctx[T] in change new in H; simpl in H
+  end.
+Local Ltac unfold_equiv :=
+  match goal with
+    | [ |- context ctx [@equiv ?A ?eq ?a ?b ]]  =>
+      let T := eval red in (@equiv A eq a b) in
+      let T := eval red in T in
+        let new := context ctx[T] in change new; simpl
+  end.
+
+Section SnakePart1.
+(** TODO: Use squares for this. (requires us to be working in a category **)
+Context {M N M' N'} `{Monoid M, Monoid N, Monoid M', Monoid N'}.
+Context (i: M→N) (i': M'→N') (f: M→M') (g: N→N').
+(** TODO: Express square using ∘ **)
+Context {Sq: ∀ m, g (i m) = i' (f m)}.
+Context `{!Monoid_Morphism i, !Monoid_Morphism i', !Monoid_Morphism f, !Monoid_Morphism g}.
+
+Program Definition KernelMap: Kernel f → Kernel g := fun m => i m.
+Next Obligation.
+  rewrite Sq.
+  destruct m as [m Hm]; simpl.
+  rewrite Hm. apply preserves_mon_unit.
+Qed.
+
+Global Instance: Proper (equiv ==> equiv) KernelMap.
+Proof.
+  intros [x Hx] [y Hy] Hxy.
+  unfold_equiv.
+  apply sm_proper; assumption.
+Qed.
+Global Instance Setoid_Morphism_instance_2: Setoid_Morphism KernelMap.
+Global Instance: SemiGroup_Morphism KernelMap.
+Proof.
+  constructor; try typeclasses eauto.
+  intros [m Hm] [n Hn].
+  unfold_equiv.
+  apply preserves_sg_op.
+Qed.
+Global Instance Monoid_Morphism_instance_1: Monoid_Morphism KernelMap.
+Proof.
+  constructor; try typeclasses eauto.
+  unfold_equiv.
+  apply preserves_mon_unit.
+Qed.
+
+Context `{!Mono i}.
+Global Instance: Mono KernelMap.
+  intros [??] ? Hm.
+  unfold_equiv in Hm .
+  apply (mono i); assumption.
+Qed.
+End SnakePart1.
+
+Section SnakePart2.
+(** FIXME: Copied from SnakePart1 **)
+Context {M N M' N'} `{AbGroup M, AbGroup N, AbGroup M', AbGroup N'}.
+Context (i: M→N) (i': M'→N') (f: M→M') (g: N→N').
+Context {Sq: ∀ m, g (i m) = i' (f m)}.
+Context `{!Monoid_Morphism i, !Monoid_Morphism i', !Monoid_Morphism f, !Monoid_Morphism g}.
+Definition CokernelMap: Cokernel f → Cokernel g := fun x => cok (i' (sec x)).
+Global Instance: Proper ((eck f) ==> (eck g)) CokernelMap.
+Proof.
+  intros [m] [n] [k Hk].
+  exists (i k). simpl.
+  rewrite Sq.
+  rewrite <- preserves_sg_op.
+  apply sm_proper; assumption.
+Qed.
+Global Instance Setoid_Morphism_instance_3: Setoid_Morphism (Aeq:=eck f) (Beq:=eck g) CokernelMap.
+Global Instance: SemiGroup_Morphism (Aeq:=eck f) (Beq:=eck g) CokernelMap.
+Proof.
+  constructor; try typeclasses eauto.
+  intros [m] [n]; exists (mon_unit:N); simpl.
+  rewrite <- preserves_sg_op.
+  rewrite preserves_mon_unit.
+  symmetry; apply left_identity.
+Qed.
+Global Instance Monoid_Morphism_2: Monoid_Morphism (Aeq:=eck f) (Beq:= eck g) CokernelMap.
+Proof.
+  constructor; try typeclasses eauto.
+  exists (mon_unit:N); simpl.
+  do 2 rewrite preserves_mon_unit.
+  symmetry; apply right_identity.
+Qed.
+End SnakePart2.
+
+Section SnakePart3.
+Context M N O M' N' O'  `{AbGroup M, AbGroup N, AbGroup O, AbGroup M', AbGroup N', AbGroup O'}.
+Context (i: M→N) (p: N→O) (i': M'→N') (p': N'→O') (f: M→M') (g: N→N') (h: O→O').
+Context {Sq_l: ∀ m, g (i m) = i' (f m)} {Sq_r: ∀ n, h (p n) = p' (g n)}.
+Context `{!Monoid_Morphism i, !Monoid_Morphism p, !Monoid_Morphism i', !Monoid_Morphism p'}.
+Context `{!Monoid_Morphism f, !Monoid_Morphism g, !Monoid_Morphism h}.
+
+Context `{!Mono i'} `{!Exact i p}.
+Global Instance: Exact (KernelMap i i' f g (Sq:=Sq_l)) (KernelMap p p' g h (Sq:=Sq_r)).
+Proof.
+  split.
+  * intros [m Hm].
+    unfold_equiv.
+    apply image_in_kernel.
+    assumption.
+  * intros [n Hn] Hn'. 
+    unfold_equiv in Hn'.
+    set (m := kernel_in_image i p n).
+    destruct m as [m Hm]; [assumption | ].
+    assert (Hm': f m = mon_unit).
+    - apply (mono_preserves_unit i').
+      rewrite <- Sq_l.
+      rewrite Hm; assumption.
+    - eexists (exist (fun m => f m = mon_unit) m Hm').
+      unfold_equiv; assumption.
+Qed.
+
+Context `{!Epi p} `{!Exact i' p'}.
+Global Instance: Exact (e0:=eck g)(e1:=eck h) (CokernelMap i' f g) (CokernelMap p' g h).
+Proof.
+  split.
+  * intros m.
+    unfold CokernelMap in *.
+    unfold_equiv.
+    exists (p mon_unit:O).
+    rewrite right_identity.
+    rewrite Sq_r.
+    erewrite (exact_equal_epi i' p').
+    exists (sec m).
+    rewrite preserves_mon_unit.
+    symmetry; apply right_identity.
+  * intros n Hn.
+    unfold CokernelMap in *.
+    unfold_equiv in Hn.
+    destruct Hn as [o Ho].
+    rewrite right_identity in Ho.
+    destruct (epi p o) as [n' Hn'].
+    rewrite <- Hn', Sq_r in Ho; clear o Hn'.
+    destruct (kernel_in_image i' p' (- (g n') & sec n)) as [m Hm].
+    rewrite preserves_sg_op, Ho, preserves_inv; try typeclasses eauto.
+    apply left_inverse.
+    exists (@cok _ _ f m).
+    unfold_equiv.
+    exists (- n').
+    rewrite preserves_inv; try typeclasses eauto.
+    assumption.
+Qed.
+
+Context {Choice: ∀ A B (f: A→B) `{Equiv B} (b: B), (∃ a:A, f a = b) → {a | f a = b}}.
+Implicit Arguments Choice [[A][B][H5]].
+
+Lemma fChoice {A B} (F: A→B) `{Equiv B} b a: F (` (Choice F b a)) = b.
+Proof.
+  set (a' := Choice F b a).
+  destruct a' as [a' Ha'].
+  apply Ha'.
+Qed.
+
+Program Definition Snake : Kernel h → Cokernel f := fun o => cok (Choice i' _ (kernel_in_image i' p' (g (Choice p o (epi p o))) _)).
+Next Obligation.
+  destruct o as [o Ho].
+  rewrite <- Sq_r. 
+  simpl. 
+  rewrite fChoice.
+  assumption.
+  Show Proof.
+Qed.
+
+Global Instance: Exact (e1:=eck f)  (KernelMap p p' g h (Sq:=Sq_r)) Snake.
+split.
+* intros [n Hn].
+  unfold_equiv. setoid_rewrite right_identity.
+  unfold Snake, KernelMap; simpl.
+  set (n' := Choice _ _ (epi p (p n))).
+  assert ((p (-n &  ` n')) = mon_unit) by (destruct n' as [n' Hn']; rewrite preserves_sg_op, preserves_inv, Hn', left_inverse; try reflexivity; typeclasses eauto).
+  destruct (kernel_in_image i p (-n & `n') H5) as [m Hm].
+  exists m.
+  apply (mono i').
+  rewrite fChoice.
+  rewrite <- Sq_l, Hm, preserves_sg_op, preserves_inv; try typeclasses eauto.
+  rewrite Hn, inv_0, left_identity.
+  reflexivity.
+* intros [o Ho]. 
+  unfold Snake.
+  simpl.
+  set (n:= Choice _ _ (epi p o)).
+  intros [m Hm].  
+  rewrite right_identity in Hm.
+  assert (g (` n & - i m) = mon_unit) by (
+    rewrite preserves_sg_op, preserves_inv; try typeclasses eauto;
+    rewrite Sq_l, <- Hm; simpl; rewrite fChoice;
+    apply right_inverse).
+  exists (exist (fun n => g n = mon_unit) (`n & - i m) H5).
+  unfold_equiv.
+  rewrite preserves_sg_op, preserves_inv; try typeclasses eauto.
+  subst n.
+  rewrite fChoice.
+  rewrite (image_in_kernel i p), inv_0.
+  apply right_identity.
+Qed.
+
+Global Instance: Exact (e0:=eck f) (e1:=eck g)  Snake (fun x => cok (i' (sec x))).
+Proof.
+split.
+* intros [o Ho]. 
+  unfold Snake. simpl.
+  rewrite fChoice.
+  simpl; set (n:= Choice _ _ (epi p o)).
+  unfold_equiv; exists (` n).
+  symmetry; apply right_identity.
+* intros m' Hm'.
+  unfold_equiv in Hm'.
+  setoid_rewrite right_identity in Hm'.
+  assert (∃ k: N, g k = i' (sec m')) by (destruct Hm' as [n Hn]; exists n; symmetry; exact Hn).
+  clear Hm'; apply Choice in H5; destruct H5 as [n Hn].
+  assert (h (p n) = mon_unit) by (rewrite Sq_r, Hn; apply image_in_kernel; typeclasses eauto).
+  exists (exist (fun o => h o = mon_unit) (p n) H5).
+  unfold Snake.
+  unfold_equiv.
+  set (n' :=  (Choice p (p n) (epi p (p n)))).
+  assert (p (`n' & -n) = mon_unit) by (destruct n' as [n' Hn']; rewrite preserves_sg_op, preserves_inv, Hn'; try apply right_inverse; typeclasses eauto).
+  set (m := Choice i _ (kernel_in_image i p (`n'&-n) H6)).
+  destruct m as [m Hm].
+  exists m.
+  apply (mono i').
+  rewrite fChoice.
+  rewrite preserves_sg_op, <- Sq_l.
+  rewrite <- Hn, <- preserves_sg_op.
+  rewrite Hm.
+  rewrite <- sg_ass, left_inverse, right_identity; try typeclasses eauto.
+  reflexivity.
+Qed.
+End SnakePart3.
+
+End Morphisms.
